vale/code/arch/x64/X64.BufferViewStore.fst
@@ -3,7 +3,6 @@ module X64.BufferViewStore
 open Views
 open Interop
 module MB = LowStar.Monotonic.Buffer
-module BV = LowStar.BufferView
 module HS = FStar.HyperStack
 open BufferViewHelpers
 open Types_s
